Weidenbach_Book/CDCL_WNOT.thy
@@ -38,9 +38,9 @@ lemma defined_lit_convert_trail_from_W[simp]:
 text \<open>The values @{term "0::nat"} and @{term "{#}"} are dummy values.\<close>
 consts dummy_cls :: 'cls
 fun convert_ann_lit_from_NOT
-  :: "('a, 'e, 'b) ann_lit \<Rightarrow> ('a, nat, 'cls) ann_lit"  where
+  :: "('a, 'e, 'b) ann_lit \<Rightarrow> ('a, unit, 'cls) ann_lit"  where
 "convert_ann_lit_from_NOT (Propagated L _) = Propagated L dummy_cls" |
-"convert_ann_lit_from_NOT (Decided L _) = Decided L 0"
+"convert_ann_lit_from_NOT (Decided L _) = Decided L ()"
 
 abbreviation convert_trail_from_NOT where
 "convert_trail_from_NOT \<equiv> map convert_ann_lit_from_NOT"
@@ -311,7 +311,7 @@ next
   then obtain L where
     undef_L: "undefined_lit (trail S) L" and
     atm_L: "atm_of L \<in> atms_of_mm (init_clss S)" and
-    T: "T \<sim> cons_trail (Decided L (Suc (backtrack_lvl S)))
+    T: "T \<sim> cons_trail (Decided L ())
       (update_backtrack_lvl (Suc (backtrack_lvl S)) S)"
     by (auto elim: decideE)
   have "decide\<^sub>N\<^sub>O\<^sub>T S T"
@@ -380,7 +380,8 @@ next
       then obtain M1 M2 i D L K where
         confl_T': "raw_conflicting T' = Some D" and
         LD: "L \<in># mset_ccls D" and
-        M1_M2:"(Decided K (i+1) # M1, M2) \<in> set (get_all_ann_decomposition (trail T'))" and
+        M1_M2:"(Decided K () # M1, M2) \<in> set (get_all_ann_decomposition (trail T'))" and
+        "get_level (trail T') K = i+1"
         "get_level (trail T') L = backtrack_lvl T'" and
         "get_level (trail T') L = get_maximum_level (trail T') (mset_ccls D)" and
         "get_maximum_level (trail T') (mset_ccls (remove_clit L D)) = i" and
@@ -425,12 +426,12 @@ next
       obtain M where tr_T: "trail T = M @ trail T'"
         using s_or_r skip_or_resolve_state_change by meson
       obtain M' where
-        tr_T': "trail T' = M' @  Decided K (i+1) # tl (trail U)" and
+        tr_T': "trail T' = M' @  Decided K () # tl (trail U)" and
         tr_U: "trail U = Propagated L (mset_ccls D) # tl (trail U)"
         using U M1_M2 undef_L inv_T' unfolding cdcl\<^sub>W_all_struct_inv_def cdcl\<^sub>W_M_level_inv_def
         by fastforce
       def M'' \<equiv> "M @ M'"
-      have tr_T: "trail S = M'' @  Decided K (i+1) # tl (trail U)"
+      have tr_T: "trail S = M'' @  Decided K () # tl (trail U)"
         using tr_T tr_T' confl unfolding M''_def by (auto elim: rulesE)
       have "init_clss T' + learned_clss S \<Turnstile>pm mset_ccls D"
         using inv_T' confl_T' unfolding cdcl\<^sub>W_all_struct_inv_def cdcl\<^sub>W_learned_clause_def
@@ -439,7 +440,7 @@ next
         reduce_trail_to M1 S"
         by (rule reduce_trail_to_length) simp
       moreover have "trail (reduce_trail_to M1 S) = M1"
-        apply (rule reduce_trail_to_skip_beginning[of _ "M @ _ @ M2 @ [Decided K (Suc i)]"])
+        apply (rule reduce_trail_to_skip_beginning[of _ "M @ _ @ M2 @ [Decided K ()]"])
         using confl M1_M2 \<open>trail T = M @ trail T'\<close>
           apply (auto dest!: get_all_ann_decomposition_exists_prepend
             elim!: conflictE)
@@ -451,7 +452,6 @@ next
         using inv_U unfolding cdcl\<^sub>W_all_struct_inv_def cdcl\<^sub>W_conflicting_def by simp
       then have U_D: "tl (trail U) \<Turnstile>as CNot (remove1_mset L (mset_ccls D))"
         by (metis append_self_conv2 tr_U)
-      thm  backjump_l[of _ _ _ _ _ L "cls_of_ccls D" _ "remove1_mset L (mset_ccls D)"]
       have "backjump_l S U"
         apply (rule backjump_l[of _ _ _ _ _ L "cls_of_ccls D" _ "remove1_mset L (mset_ccls D)"])
                  using tr_T apply simp
